Commit pre-redéfinition égalité Maps

.CoqMakefile.d
@@ -4,6 +4,9 @@ src/Canonical_form.vos src/Canonical_form.vok src/Canonical_form.required_vos: s
 src/Closed.vo src/Closed.glob src/Closed.v.beautified src/Closed.required_vo: src/Closed.v src/Hints.vo src/Syntax.vo src/Types.vo src/Maps.vo
 src/Closed.vio: src/Closed.v src/Hints.vio src/Syntax.vio src/Types.vio src/Maps.vio
 src/Closed.vos src/Closed.vok src/Closed.required_vos: src/Closed.v src/Hints.vos src/Syntax.vos src/Types.vos src/Maps.vos
+src/Eval.vo src/Eval.glob src/Eval.v.beautified src/Eval.required_vo: src/Eval.v src/Types.vo src/Syntax.vo src/Step.vo src/Subst.vo src/Hints.vo src/Closed.vo src/Multi.vo
+src/Eval.vio: src/Eval.v src/Types.vio src/Syntax.vio src/Step.vio src/Subst.vio src/Hints.vio src/Closed.vio src/Multi.vio
+src/Eval.vos src/Eval.vok src/Eval.required_vos: src/Eval.v src/Types.vos src/Syntax.vos src/Step.vos src/Subst.vos src/Hints.vos src/Closed.vos src/Multi.vos
 src/Hints.vo src/Hints.glob src/Hints.v.beautified src/Hints.required_vo: src/Hints.v 
 src/Hints.vio: src/Hints.v 
 src/Hints.vos src/Hints.vok src/Hints.required_vos: src/Hints.v 
@@ -28,6 +31,9 @@ src/Subst.vos src/Subst.vok src/Subst.required_vos: src/Subst.v src/Closed.vos s
 src/Syntax.vo src/Syntax.glob src/Syntax.v.beautified src/Syntax.required_vo: src/Syntax.v src/Maps.vo src/Hints.vo
 src/Syntax.vio: src/Syntax.v src/Maps.vio src/Hints.vio
 src/Syntax.vos src/Syntax.vok src/Syntax.required_vos: src/Syntax.v src/Maps.vos src/Hints.vos
+src/Transformations/Pair_Records.vo src/Transformations/Pair_Records.glob src/Transformations/Pair_Records.v.beautified src/Transformations/Pair_Records.required_vo: src/Transformations/Pair_Records.v src/Maps.vo src/Syntax.vo src/Step.vo src/Subst.vo src/Hints.vo src/Closed.vo src/Types.vo
+src/Transformations/Pair_Records.vio: src/Transformations/Pair_Records.v src/Maps.vio src/Syntax.vio src/Step.vio src/Subst.vio src/Hints.vio src/Closed.vio src/Types.vio
+src/Transformations/Pair_Records.vos src/Transformations/Pair_Records.vok src/Transformations/Pair_Records.required_vos: src/Transformations/Pair_Records.v src/Maps.vos src/Syntax.vos src/Step.vos src/Subst.vos src/Hints.vos src/Closed.vos src/Types.vos
 src/Types.vo src/Types.glob src/Types.v.beautified src/Types.required_vo: src/Types.v src/Hints.vo src/Maps.vo src/Syntax.vo
 src/Types.vio: src/Types.v src/Hints.vio src/Maps.vio src/Syntax.vio
 src/Types.vos src/Types.vok src/Types.required_vos: src/Types.v src/Hints.vos src/Maps.vos src/Syntax.vos
