src/Closed.v
@@ -8,69 +8,58 @@ Require Import Types.
 Require Maps.
 Import Maps.Notations.
 
-(* 
-Variable libre:
-x libre dans e si 
-e = Var x
-e = App e1 e2 => x libre dans e1 ou x libre dans e2
-e = λ y : t . e => y <> x et x libre dans e
-e = If e1 e2 e3 => x libre dans e1 ou x libre dans e2 ou x libre dans e3
-e = Let y e1 e2 => x libre dans e1 ou x <> y et x libre dans e2
-e = Minus e1 e2 => x libre dans e1 ou x libre dans e2
- *)
-
 Inductive is_free_in (x : string) : expr -> Prop :=
-  | Free_Var : is_free_in x (E_Var x)
+  | Free_Var : is_free_in x <{x}>
   | Free_App_Left : 
       ∀ e₁ e₂, 
       is_free_in x e₁ -> 
-      is_free_in x (E_App e₁ e₂) 
+      is_free_in x <{e₁ e₂}>
   | Free_App_Right : 
       ∀ e₁ e₂, 
       is_free_in x e₂ -> 
-      is_free_in x (E_App e₁ e₂) 
+      is_free_in x <{e₁ e₂}>
   | Free_Fun : 
       ∀ y t e, 
       y <> x -> 
       is_free_in x e -> 
-      is_free_in x (E_Fun y t e) 
+      is_free_in x <{fun y : t => e}> 
   | Free_If_Cond : 
       ∀ e₁ e₂ e₃, 
       is_free_in x e₁ -> 
-      is_free_in x (E_If e₁ e₂ e₃) 
+      is_free_in x <{if e₁ then e₂ else e₃}> 
   | Free_If_Left : 
       ∀ e₁ e₂ e₃, 
       is_free_in x e₂ -> 
-      is_free_in x (E_If e₁ e₂ e₃) 
+      is_free_in x <{if e₁ then e₂ else e₃}> 
   | Free_If_Right : 
       ∀ e₁ e₂ e₃, 
       is_free_in x e₃ -> 
-      is_free_in x (E_If e₁ e₂ e₃) 
+      is_free_in x <{if e₁ then e₂ else e₃}> 
   | Free_Let_Left : 
       ∀ y e₁ e₂, 
       is_free_in x e₁ -> 
-      is_free_in x (E_Let y e₁ e₂) 
+      is_free_in x <{let y = e₁ in e₂}>
   | Free_Let_Right : 
       ∀ y e₁ e₂, 
       y <> x -> is_free_in x e₂ -> 
-      is_free_in x (E_Let y e₁ e₂) 
+      is_free_in x <{let y = e₁ in e₂}>
   | Free_Minus_Left : 
       ∀ e₁ e₂, 
       is_free_in x e₁ -> 
-      is_free_in x (E_Minus e₁ e₂) 
+      is_free_in x <{e₁ - e₂}>
   | Free_Minus_Right : 
       ∀ e₁ e₂, 
       is_free_in x e₂ -> 
-      is_free_in x (E_Minus e₁ e₂)
+      is_free_in x <{e₁ - e₂}>
 
   | Free_Eq_Left : 
       ∀ e₁ e₂, 
       is_free_in x e₁ -> 
-      is_free_in x (E_Eq e₁ e₂) 
+      is_free_in x <{e₁ == e₂}>
   | Free_Eq_Right : 
       ∀ e₁ e₂, 
       is_free_in x e₂ -> 
-      is_free_in x (E_Eq e₁ e₂)  
+      is_free_in x <{e₁ == e₂}>
   | Free_Pair_Left : 
       ∀ e₁ e₂, 
       is_free_in x e₁ -> 
@@ -102,47 +91,81 @@ Inductive is_free_in (x : string) : expr -> Prop :=
       is_free_in x e -> 
       is_free_in x (E_Record_Access e y) 
 
-  | Free_Fix :
-    ∀ e, 
+  | Free_Fix :  
+      ∀ e, 
       is_free_in x e -> 
       is_free_in x (E_Fix e) 
+
+  | Free_In_Left :
+      ∀ e t₁ t₂, 
+      is_free_in x e ->
+      is_free_in x (E_In_Left t₁ t₂ e)
+  
+  | Free_In_Right :
+      ∀ e t₁ t₂, 
+      is_free_in x e -> 
+      is_free_in x (E_In_Right t₁ t₂ e)
+
+  | Free_Match_Main :
+      ∀ e e_left e_right, 
+      is_free_in x e -> 
+      is_free_in x (E_Match e e_left e_right)
+
+  | Free_Match_Left :
+      ∀ e e_left e_right, 
+      is_free_in x e_left -> 
+      is_free_in x (E_Match e e_left e_right)
+  
+  | Free_Match_Right :
+      ∀ e e_left e_right, 
+      is_free_in x e_right -> 
+      is_free_in x (E_Match e e_left e_right)
+  | Free_Sum_Constr :
+      ∀ e constr, 
+      is_free_in x e -> 
+      is_free_in x (E_Sum_Constr constr e)
 .
 
 Hint Constructors is_free_in : local_hints.
 
-Definition closed e := ∀ x, ~ is_free_in x e.
+Definition closed e := ∀ x, ¬ is_free_in x e.
+
+Hint Unfold closed : local_hints.
 
 Lemma free_has_type :
-    ∀ Γ e t x,
+    ∀ Γ Σ e t x,
     is_free_in x e ->
-    Γ ⊢ e ∈ t -> 
+    has_type Σ Γ  e  t ->  
     ∃ t_x, Γ ? x = Some t_x.
 Proof.
   intros * H_free H_type.
   generalize dependent Γ.
   generalize dependent t.
   induction H_free; intros;
-  try (inversion H_type; subst; try eauto; fail);
-  try (inversion H_type; subst; erewrite <- Maps.update_neq; eauto; fail).
+  inversion H_type; subst; eauto;
+  erewrite <- Maps.update_neq; eauto.
 Qed. 
 
 Hint Resolve free_has_type : local_hints.
 
 
 Theorem typed_empty :
-    ∀ e t,
-    empty ⊢ e ∈ t -> 
+    ∀ Σ e t,
+    has_type Σ empty  e  t ->  
     closed e.
 Proof.
     intros * H_type x H_contra.
     generalize dependent t.
     induction H_contra; intros;
     try (inversion H_type; subst; eauto; fail).
-    - inversion H_type; subst. inversion H1.
-    - inversion H_type; subst. 
-      eapply free_has_type in H_contra; eauto.
-      inversion H_contra. rewrite Maps.update_neq in H0; eauto. inversion H0.
-    - inversion H_type; subst. 
+    - (* e = E_Var x *) 
+      inversion H_type; subst. inversion H2.
+    - (* e = E_fun y t e', x != y *)
+      inversion H_type; subst. 
+      eapply free_has_type with (Γ := (y |-> t; empty)) (t := t2) in H_contra as [t_x H_eq]; eauto.
+      rewrite Maps.update_neq in H_eq; eauto. inversion H_eq.
+    - (* e = E_let y e₁ e₂, x != y *) 
+      inversion H_type; subst. 
       eapply free_has_type in H_contra; eauto.
       inversion H_contra. 
       rewrite Maps.update_neq in H0; eauto. inversion H0.
@@ -190,7 +213,7 @@ Lemma closed_if :
 Proof.
   intros.
   unfold closed in *.
-  repeat split; 
+  repeat split;
     intros x H_contra;
     apply H with x;
     eauto with local_hints.
@@ -270,8 +293,6 @@ Proof.
   apply H with x';
   eauto with local_hints.
 Qed.
-
-
 Hint Resolve closed_second : local_hints.
 
 
@@ -287,7 +308,6 @@ Proof.
     apply H with x';
     eauto with local_hints.
 Qed.
-
 Hint Resolve closed_record : local_hints.
 
 
@@ -302,6 +322,8 @@ Proof.
   apply H with x';
   eauto with local_hints.
 Qed.
+Hint Resolve closed_access : local_hints.
+
 
 Lemma closed_fix : 
   ∀ e, 
@@ -314,5 +336,60 @@ Proof.
   apply H with x';
   eauto with local_hints.
 Qed.
+Hint Resolve closed_fix : local_hints.
 
-Hint Resolve closed_access : local_hints.
+
+Lemma closed_in_left :
+  ∀ e t₁ t₂,
+  closed (E_In_Left t₁ t₂ e) ->  
+  closed e.
+Proof.
+  intros.
+  unfold closed in *.
+  intros x' H_contra;
+  apply H with x';
+  eauto with local_hints.
+Qed.
+Hint Resolve closed_in_left : local_hints.
+
+Lemma closed_in_right :
+  ∀ e t₁ t₂,
+  closed (E_In_Right t₁ t₂ e) ->  
+  closed e.
+Proof.
+  intros.
+  unfold closed in *.
+  intros x' H_contra;
+  apply H with x';
+  eauto with local_hints.
+Qed.
+Hint Resolve closed_in_right : local_hints.
+
+
+
+Lemma closed_match :
+  ∀ e e_left e_right,
+  closed (E_Match e e_left e_right) -> 
+  closed e /\ closed e_left /\ closed e_right.
+Proof.
+  intros.
+  unfold closed in *.
+  repeat split;
+    intros x' H_contra;
+    apply H with x';
+    eauto with local_hints.
+Qed.
+Hint Resolve closed_match : local_hints.
+
+Lemma closed_sum_constr :
+  ∀ constr e,
+  closed (E_Sum_Constr constr e) -> 
+  closed e.
+Proof.
+  intros.
+  unfold closed in *.
+    intros x' H_contra;
+    apply H with x';
+    eauto with local_hints.
+Qed.
+Hint Resolve closed_sum_constr : local_hints.
