src/Multi.v
@@ -1,5 +1,4 @@
 From Coq Require Import Unicode.Utf8.
-From Coq Require Import Relation_Definitions.
 Require Import Syntax.
 Require Import Step.
 Require Import Subst.
@@ -11,35 +10,33 @@ Require Import Lia.
 Require Import String.
 
 
-Reserved Notation "e1 ->>* e2" (at level 70, no associativity) .
+Reserved Notation "e₁ -->* e₂" (at level 70, no associativity) .
 
 Inductive multistep : expr -> expr -> Prop :=
-  | multistep_step : 
-      ∀ e1 e2, 
-      e1 ->> e2 -> 
-      e1 ->>* e2 
   | multistep_refl : 
       ∀ e, 
-      e ->>* e 
+      e -->* e 
+  | multistep_step : 
+      ∀ e₁ e₂, 
+      e₁ --> e₂ -> 
+      e₁ -->* e₂ 
   | multistep_trans :
       ∀ x y z,
-      x ->>* y -> 
-      y ->>* z -> 
-      x ->>* z 
-  where "e1 ->>* e2" := (multistep e1 e2)
-  .
+      x -->* y -> 
+      y -->* z -> 
+      x -->* z 
+  where "e₁ -->* e₂" := (multistep e₁ e₂)
+. 
+Check multistep_ind.
+
+(* 
+  TODO: Prouver équivalence avec une définition algorithmique + définir Induction par la gauche et la droite
+*)
 
 Hint Constructors multistep : local_hints.
 
-Lemma multistep_step_ : ∀ e1 e2, e1 ->> e2 -> e1 ->>* e2.
-Proof.
-  eauto with local_hints.
-  Show Proof.
-Qed.
-
-
 Example multistep_if :
-  <{if 1 == 2 then 3 else 0}> ->>* <{0}>.
+  <{if 1 == 2 then 3 else 0}> -->* <{0}>.
 Proof.
   eauto 6 with zarith local_hints.
 Qed.
@@ -62,103 +59,7 @@ Definition inner_eq := <{
 }>.
 
 
-Example multistep_fix : 
-<{
-  (fix inner_eq) 1 1
-}> ->>* <{true}>.
-Proof with eauto 8 with zarith local_hints.
-  assert (H_closed_fun_eq : 
-    closed (E_Fix inner_eq)
-  ).
-  {
-    unfold inner_eq.
-    intros x H_n.
-      inversion H_n.
-      inversion H0.
-      inversion H5; subst.
-      inversion H10; subst.
-      inversion H6; subst;
-      try (
-        inversion H1; subst;
-        inversion H4; subst; eauto; fail
-      ).
-      inversion H1; subst; inversion H4; subst; inversion H7; subst; eauto; inversion H9; subst; eauto; inversion H11; subst; eauto.
-  }
-  assert (eq <> n). {
-    intro; inversion H.
-  }
-  assert (eq <> m). {
-    intro; inversion H0.
-  }
-  assert (n <> m). {
-    intro; inversion H1.
-  }
-  assert (closed 1). {
-    intros x Hc; inversion Hc.
-  }
-  assert (closed 0). {
-    intros x Hc; inversion Hc.
-  }
-  eapply multistep_trans.
-  - apply multistep_step. repeat apply ST_App_Left.
-    apply ST_Fix_Fun.
-    repeat apply S_Fun_Neq... 
-    repeat apply S_If...
-  - eapply multistep_trans.
-    + apply multistep_step. apply ST_App_Left.
-      apply ST_App_Fun;
-      try apply S_Fun_Neq;
-      repeat apply S_If...
-    + eapply multistep_trans.
-      * apply multistep_step. apply ST_App_Fun...
-        repeat apply S_If...
-      * {
-      eapply multistep_trans.
-      - apply multistep_step. apply ST_If...
-      - eapply multistep_trans.  
-        + apply multistep_step. apply ST_If_False.
-        + eapply multistep_trans.  
-          * apply multistep_step. apply ST_If...
-          * {
-            eapply multistep_trans.
-            - apply multistep_step. apply ST_If_False...
-            - eapply multistep_trans.
-              + apply multistep_step. repeat apply ST_App_Left.
-                apply ST_Fix_Fun.
-                repeat apply S_Fun_Neq... 
-                repeat apply S_If...
-              + eapply multistep_trans.
-                * apply multistep_step. apply ST_App_Left.
-                  apply ST_App_Right...
-                * {
-                  eapply multistep_trans.
-                  - apply multistep_step. apply ST_App_Left.
-                    simpl.
-                    apply ST_App_Fun...
-                    apply S_Fun_Neq...
-                    repeat apply S_If...
-                  - eapply multistep_trans.
-                    + apply multistep_step. apply ST_App_Right...
-                    + simpl.
-                      eapply multistep_trans.
-                      * apply multistep_step. 
-                        eapply ST_App_Fun...
-                        repeat apply S_If...
-                      * {
-                      eapply multistep_trans.
-                      - apply multistep_step...
-                      - eapply multistep_trans... 
-                      }
-                      
-                }
-          } 
-      }
-Qed.
-
-Example multistep_fix' : 
-<{
-  (fix inner_eq) 1 1
-}> ->>* <{true}>.
+Goal <{(fix inner_eq) 1 1}> -->* <{true}>.
 Proof with eauto 8 with zarith local_hints.
   assert (H_closed_fun_eq : 
     closed (E_Fix inner_eq)
@@ -201,7 +102,7 @@ Proof with eauto 8 with zarith local_hints.
     apply ST_Fix_Fun.
     repeat apply S_Fun_Neq... 
     repeat apply S_If...
-  - apply multistep_step... apply ST_App_Left. 
+  - apply multistep_step. apply ST_App_Left. 
     apply ST_App_Fun;
     try apply S_Fun_Neq;
     try repeat apply S_If...
@@ -233,3 +134,36 @@ Proof with eauto 8 with zarith local_hints.
   - apply multistep_step...  
   - apply multistep_refl. 
 Qed.
+
+Check multistep_ind. 
+
+
+(* TODO:
+    prouver que x --> y -> P x y -> x -->* y -> P x y ou similaire
+ *)
+Lemma exists_red : ∀ x y, x -->* y -> x = y \/ ∃ aux, x --> aux /\ aux -->* y.
+Proof with eauto with local_hints.
+  intros.
+  induction H...
+  destruct IHmultistep1 as [ H_x_eq_y | [x_aux [H_x_red H_xaux_red]]];
+  destruct IHmultistep2 as [ H_y_eq_z | [y_aux [H_y_red H_yaux_red]]]; subst...
+Qed.
+
+Hint Resolve exists_red : local_hints.
+
+Theorem multistep_step_multistep :
+  ∀ x y z, x --> y -> y -->* z -> x -->* z.
+Proof with eauto with local_hints.
+  intros.
+  apply multistep_trans with y...
+Qed.
+
+Check multistep_ind.
+
+
+Theorem multistep_ind_left (P : expr -> expr -> Prop) :
+  (∀ e : expr, P e e) → 
+  (∀ x y z : expr, x --> y → y -->* z → P y z → P x z) → 
+  ∀ e e' : expr, e -->* e' → P e e'.
+Proof with eauto with local_hints.
+Admitted.
