src/Step.v
@@ -9,135 +9,182 @@ Require Import Subst.
 Require Maps.
 Import Maps.Notations.
 
-Reserved Notation "x ->> y" (at level 70, no associativity).
+Reserved Notation "x --> y" (at level 70, no associativity).
 
 Inductive step : expr -> expr -> Prop := 
   | ST_App_Fun : 
       ∀ (x : string) (t : type) (e e' v : expr),
       value v -> 
       substitution v x e e' ->
-      (E_App (E_Fun x t e) v) ->> e'
+      (E_App (E_Fun x t e) v) --> e'
   | ST_App_Left : 
       ∀ (e1 e1' e2 : expr),
-      e1 ->> e1' ->
-      (E_App e1 e2) ->> (E_App e1' e2)
+      e1 --> e1' ->
+      (E_App e1 e2) --> (E_App e1' e2)
   | ST_App_Right : 
       ∀ (v1 e2 e2' : expr),
       value v1 ->
-      e2 ->> e2' ->
-      (E_App v1 e2) ->> (E_App v1 e2')
+      e2 --> e2' ->
+      (E_App v1 e2) --> (E_App v1 e2')
   | ST_If_True : 
       ∀ (e1 e2 : expr),
-      (E_If E_True e1 e2) ->> e1
+      (E_If E_True e1 e2) --> e1
   | ST_If_False : 
       ∀ (e1 e2 : expr),
-      (E_If E_False e1 e2) ->> e2
+      (E_If E_False e1 e2) --> e2
   | ST_If : 
       ∀ (e1 e1' e2 e3 : expr),
-      e1 ->> e1' ->
-      (E_If e1 e2 e3) ->> (E_If e1' e2 e3)
+      e1 --> e1' ->
+      (E_If e1 e2 e3) --> (E_If e1' e2 e3)
   | ST_Let_Left : 
       ∀ (x : string) (e1 e1' e2 : expr),
-      e1 ->> e1' ->
-      (E_Let x e1 e2) ->> (E_Let x e1' e2)
+      e1 --> e1' ->
+      (E_Let x e1 e2) --> (E_Let x e1' e2)
   | ST_Let_Right : 
       ∀ (x : string) (v1 e2 e2' : expr),
       value v1 ->
       substitution v1 x e2 e2' ->
-      (E_Let x v1 e2) ->> e2'
+      (E_Let x v1 e2) --> e2'
   | ST_Minus_Left :  
       ∀ (e1 e1' e2 : expr),
-      e1 ->> e1' ->
-      (E_Minus e1 e2) ->> (E_Minus e1' e2)
+      e1 --> e1' ->
+      (E_Minus e1 e2) --> (E_Minus e1' e2)
   | ST_Minus_Right :  
       ∀ (v1 e2 e2' : expr),
       value v1 ->
-      e2 ->> e2' ->
-      (E_Minus v1 e2) ->> (E_Minus v1 e2')
+      e2 --> e2' ->
+      (E_Minus v1 e2) --> (E_Minus v1 e2')
   | ST_Minus_Num : 
       ∀ (z1 z2 : Z),
-      (E_Minus (E_Num z1) (E_Num z2)) ->> (E_Num (z1 - z2))
+      (E_Minus (E_Num z1) (E_Num z2)) --> (E_Num (z1 - z2))
 
   | ST_Eq_Left :  
       ∀ (e1 e1' e2 : expr),
-      e1 ->> e1' ->
-      (E_Eq e1 e2) ->> (E_Eq e1' e2)
+      e1 --> e1' ->
+      (E_Eq e1 e2) --> (E_Eq e1' e2)
   | ST_Eq_Right :  
       ∀ (v1 e2 e2' : expr),
       value v1 ->
-      e2 ->> e2' ->
-      (E_Eq v1 e2) ->> (E_Eq v1 e2')
+      e2 --> e2' ->
+      (E_Eq v1 e2) --> (E_Eq v1 e2')
   | ST_Eq_Num_Eq : 
       ∀ (z : Z),
-      (E_Eq (E_Num z) (E_Num z)) ->> (E_True)
+      (E_Eq (E_Num z) (E_Num z)) --> (E_True)
   | ST_Eq_Num_Neq : 
       ∀ (z1 z2 : Z),
       z1 <> z2 ->
-      (E_Eq (E_Num z1) (E_Num z2)) ->> (E_False)
+      (E_Eq (E_Num z1) (E_Num z2)) --> (E_False)
 
 
   | ST_Pair_Left :  
       ∀ (e1 e1' e2 : expr),
-      e1 ->> e1' ->
-      (E_Pair e1 e2) ->> (E_Pair e1' e2)
+      e1 --> e1' ->
+      (E_Pair e1 e2) --> (E_Pair e1' e2)
   | ST_Pair_Right :  
       ∀ (v1 e2 e2' : expr),
       value v1 ->
-      e2 ->> e2' ->
-      (E_Pair v1 e2) ->> (E_Pair v1 e2')
+      e2 --> e2' ->
+      (E_Pair v1 e2) --> (E_Pair v1 e2')
   | ST_First :  
       ∀ (e e' : expr),
-      e ->> e' ->
-      (E_First e) ->> (E_First e')
+      e --> e' ->
+      (E_First e) --> (E_First e')
   | ST_Second :  
       ∀ (e e' : expr),
-      e ->> e' ->
-      (E_Second e) ->> (E_Second e')
+      e --> e' ->
+      (E_Second e) --> (E_Second e')
   | ST_First_Pair :  
       ∀ (v₁ v₂ : expr),
       value v₁ -> 
       value v₂ ->
-      (E_First (E_Pair v₁ v₂)) ->> v₁
+      (E_First (E_Pair v₁ v₂)) --> v₁
   | ST_Second_Pair :  
       ∀ (v₁ v₂ : expr),
       value v₁ -> 
       value v₂ ->
-      (E_Second (E_Pair v₁ v₂)) ->> v₂
+      (E_Second (E_Pair v₁ v₂)) --> v₂
   
   | ST_Record_Tail : 
       ∀ x e tail tail', 
-      tail ->> tail' -> 
-      (E_Record_Cons x e tail) ->> (E_Record_Cons x e tail')
+      value e -> 
+      tail --> tail' -> 
+      (E_Record_Cons x e tail) --> (E_Record_Cons x e tail')
   
   | ST_Record : 
       ∀ x e e' tail,
-      value tail -> 
-      e ->> e' -> 
-      (E_Record_Cons x e tail) ->> (E_Record_Cons x e' tail)
+      e --> e' -> 
+      (E_Record_Cons x e tail) --> (E_Record_Cons x e' tail)
   
   | ST_Access : 
       ∀ x e e',
-      e ->> e' ->
-      (E_Record_Access e x) ->> (E_Record_Access e' x)
+      e --> e' ->
+      (E_Record_Access e x) --> (E_Record_Access e' x)
 
   | ST_Access_Value : 
       ∀ x e v,
       value e -> 
       lookup_val_record x e = Some v ->
-      (E_Record_Access e x) ->> v
+      (E_Record_Access e x) --> v
 
   | ST_Fix :
       ∀ (e e': expr),
-      e ->> e' ->
-      (E_Fix e) ->> (E_Fix e')
+      e --> e' ->
+      (E_Fix e) --> (E_Fix e')
   
   | ST_Fix_Fun :
       ∀ x t e e',
       substitution (E_Fix (E_Fun x t e)) x e e' ->
-      (E_Fix (E_Fun x t e)) ->> e'
+      (E_Fix (E_Fun x t e)) --> e'
 
+  | ST_In_Left :
+      ∀ t₁ t₂ e e', 
+      e --> e' -> 
+      E_In_Left t₁ t₂ e --> E_In_Left t₁ t₂ e'
+
+  | ST_In_Right :
+      ∀ t₁ t₂ e e', 
+      e --> e' -> 
+      E_In_Right t₁ t₂ e --> E_In_Right t₁ t₂ e'
+  
+  | ST_Match_Main :
+      ∀ e e' e_left e_right,
+      e --> e' ->
+      E_Match e e_left e_right --> E_Match e' e_left e_right
+
+
+  | ST_Match_Left :
+      ∀ e e_left e_left' e_right,
+      value e ->
+      e_left --> e_left' -> 
+      E_Match e e_left e_right --> E_Match e e_left' e_right
+
+  | ST_Match_Right :
+      ∀ e e_left e_right e_right',
+      value e -> 
+      value e_left -> 
+      e_right --> e_right' -> 
+      E_Match e e_left e_right --> E_Match e e_left e_right'
+
+  | ST_Match_Left_App :
+      ∀ t₁ t₂ e e_left e_right,
+      value e -> 
+      value e_left -> 
+      value e_right -> 
+      E_Match (E_In_Left t₁ t₂ e) e_left e_right --> E_App e_left e
+
+  | ST_Match_Right_App :
+    ∀ t₁ t₂ e e_left e_right,
+    value e -> 
+    value e_left -> 
+    value e_right -> 
+    E_Match (E_In_Right t₁ t₂ e) e_left e_right --> E_App e_right e
+
+  | ST_Sum_Constr :
+      ∀ constr e e',
+      e --> e' -> 
+      E_Sum_Constr constr e --> E_Sum_Constr constr e'
 where 
-    "x ->> y" := (step x y)
+    "x --> y" := (step x y)
 .
 
 Hint Constructors step : local_hints.
@@ -147,25 +194,30 @@ Hint Constructors step : local_hints.
 Local Lemma not_value: 
   ∀ e e',
   value e -> 
-  ~ e ->> e'.
+  ¬ e --> e'.
 Proof.
   induction e; intros e' H_val H_contra;
   try (inversion H_val; inversion H_contra; fail).
-  inversion H_val; subst.
-  inversion H_contra; subst.
-  - apply IHe1 with e1'; auto.
-  - apply IHe2 with e2'; auto.
+  - inversion H_val; inversion H_contra; subst.
+    + eapply IHe1; eassumption.
+    + eapply IHe2; eassumption.
   - inversion H_val; subst; inversion H_contra; subst.
-    + eapply IHe2; eauto.
-    + eapply IHe1; eauto.
+    + eapply IHe2; eassumption.
+    + eapply IHe1; eassumption.
+  - inversion H_val; inversion H_contra; subst.
+    eapply IHe; eassumption.
+  - inversion H_val; inversion H_contra; subst.
+    eapply IHe; eassumption.
+  - inversion H_val; inversion H_contra; subst.
+    eapply IHe; eassumption.
 Qed.
 
 
 
 Local Theorem deterministic :
     ∀ e e'₁ e'₂, 
-    e ->> e'₁ ->
-    e ->> e'₂ ->
+    e --> e'₁ ->
+    e --> e'₂ ->
     e'₁ = e'₂.
 Proof with eauto with local_hints.
   induction e; 
@@ -331,4 +383,45 @@ Proof with eauto with local_hints.
     + inversion H_s_1; subst. inversion H2. inversion H0.
     + inversion H2; subst.
       eapply Subst.deterministic...    
+  - inversion H_s_1; inversion H_s_2; subst.
+    specialize IHe with e' e'0. apply IHe in H3; subst; auto.
+  - inversion H_s_1; inversion H_s_2; subst.
+    specialize IHe with e' e'0. apply IHe in H3; subst; auto.
+  - inversion H_s_1; subst.
+    + inversion H_s_2; subst.
+      * specialize IHe1 with e' e'0. rewrite IHe1; auto. 
+      * apply not_value with (e':=e') in H4; contradiction.
+      * apply not_value with (e':=e') in H2; contradiction.
+      * inversion H3; subst.
+        apply not_value with (e':=e'0) in H2; contradiction.
+      * inversion H3; subst.
+        apply not_value with (e':=e'0) in H2; contradiction.
+
+    + inversion H_s_2; subst.
+      * apply not_value with (e':=e') in H3; contradiction.  
+      * specialize IHe2 with e_left' e_left'0. rewrite IHe2; auto.
+      * apply not_value with (e':=e_left') in H6; contradiction.
+      * apply not_value with (e':=e_left') in H6; contradiction.
+      * apply not_value with (e':=e_left') in H6; contradiction.  
+
+    + inversion H_s_2; subst.
+      * apply not_value with (e':=e') in H2; contradiction.  
+      * apply not_value with (e':=e_left') in H4; contradiction.
+      * specialize IHe3 with e_right' e_right'0. rewrite IHe3; auto.
+      * apply not_value with (e':=e_right') in H8; contradiction.  
+      * apply not_value with (e':=e_right') in H8; contradiction.  
+
+    + inversion H_s_2; subst.
+      * inversion H6; subst.
+        apply not_value with (e':=e'0) in H2; contradiction.
+      * apply not_value with (e':=e_left') in H4; contradiction.
+      * apply not_value with (e':=e_right') in H5; contradiction.
+      * reflexivity.
+    + inversion H_s_2; subst.
+      * inversion H6; subst.
+        apply not_value with (e':=e'0) in H2; contradiction.
+      * apply not_value with (e':=e_left') in H4; contradiction.
+      * apply not_value with (e':=e_right') in H5; contradiction.
+      * reflexivity.
+  - inversion H_s_1. inversion H_s_2; subst. f_equal. eauto.
 Qed.
