src/Types.v
@@ -3,119 +3,193 @@ Require Import Hints.
 Require Maps.
 Import Maps.Notations.
 Require Import Syntax.
+Require Import String.
+Require Import List.
+Import ListNotations.
 
 Definition context := @Maps.map type.
 Definition empty := @Maps.empty type.
+Definition sum_types_constructors : Set := 
+    list (string * list (type * string)).
+
+Fixpoint lookup_type_constrs (constr : string) (constrs : list (type * string)) : option type := 
+    match constrs with 
+    | [] => None
+    | h::t => 
+        if (snd h =? constr)%string 
+        then Some (fst h) 
+        else lookup_type_constrs constr t 
+    end.
 
 
 
-Reserved Notation "Γ '⊢' e '∈' τ" (at level 70, right associativity).
+Fixpoint lookup_type_sum (constr : string) (Σ : sum_types_constructors)
+    : option (string * type) :=
+    match Σ with 
+    | [] => None 
+    | h::Σ' => 
+        match lookup_type_constrs constr (snd h)  with 
+        | None => lookup_type_sum constr Σ'
+        | Some t => Some (fst h, t) 
+        end
+    end.
 
-Inductive has_type : context -> expr -> type -> Prop := 
+Fixpoint expected_parameter 
+  (constrs : list (type * string)) 
+  (branches : list (string * expr)) : (list (string * expr * option type)) :=
+  match branches with 
+  | [] => []
+  | h::branches' => 
+    let name := fst h in 
+    let e := snd h in 
+    let t := lookup_type_constrs name constrs in 
+    (name, e, t)::(expected_parameter constrs branches')
+  end.
+
+
+Inductive has_type : sum_types_constructors -> context -> expr -> type -> Prop := 
   (* Base λ-calculus *)
   | T_Var: 
-      ∀ Γ x t, 
+      ∀ Γ Σ x t, 
       Γ ? x = Some t -> 
-      (Γ ⊢ (E_Var x) ∈ t)
-
+      has_type Σ Γ (E_Var x) t 
   | T_Fun: 
-      ∀ Γ x t1 e (t2 : type),
-      (x |-> t1; Γ) ⊢ e ∈ t2 ->
-      Γ ⊢ (E_Fun x t1 e) ∈ (Type_Fun t1 t2)
+      ∀ Γ Σ x t1 e (t2 : type),
+      has_type Σ (x |-> t1; Γ)  e  t2 -> 
+      has_type Σ Γ  (E_Fun x t1 e)  (Type_Fun t1 t2) 
 
   | T_App: 
-      ∀ Γ e1 e2 t1 t2, 
-      Γ ⊢ e2 ∈ t1 -> 
-      Γ ⊢ e1 ∈ (Type_Fun t1 t2) ->
-      Γ ⊢ (E_App e1 e2) ∈ t2
+      ∀ Γ Σ e1 e2 t1 t2, 
+      has_type Σ Γ  e2  t1 ->  
+      has_type Σ Γ  e1  (Type_Fun t1 t2) -> 
+      has_type Σ Γ  (E_App e1 e2)  t2 
 
   (* Booleans and conditions *)
   | T_True: 
-      ∀ Γ, 
-      Γ ⊢ E_True ∈ Type_Bool
+      ∀ Γ Σ, 
+      has_type Σ Γ  E_True  Type_Bool 
               
   | T_False: 
-      ∀ Γ, 
-      Γ ⊢ E_False ∈ Type_Bool
+      ∀ Γ Σ, 
+      has_type Σ Γ  E_False  Type_Bool 
 
   | T_If: 
-      ∀ Γ e1 e2 e3 t, 
-      Γ ⊢ e1 ∈ Type_Bool -> 
-      Γ ⊢ e2 ∈ t -> 
-      Γ ⊢ e3 ∈ t -> 
-      Γ ⊢ (E_If e1 e2 e3) ∈ t 
+      ∀ Γ Σ e1 e2 e3 t, 
+      has_type Σ Γ  e1  Type_Bool ->  
+      has_type Σ Γ  e2  t ->  
+      has_type Σ Γ  e3  t ->  
+      has_type Σ Γ  (E_If e1 e2 e3)  t  
 
   (* Let expressions *)
   | T_Let : 
-      ∀ Γ x e1 e2 t1 t2, 
-      Γ ⊢ e1 ∈ t1 -> 
-      (x |-> t1; Γ) ⊢ e2 ∈ t2 -> 
-      Γ ⊢ (E_Let x e1 e2) ∈ t2
+      ∀ Γ Σ x e1 e2 t1 t2, 
+      has_type Σ Γ  e1  t1 ->  
+      has_type Σ (x |-> t1; Γ)  e2  t2 ->  
+      has_type Σ Γ  (E_Let x e1 e2)  t2 
 
   (* Arithmetic *)
   | T_Num : 
-      ∀ Γ z, 
-      Γ ⊢ (E_Num z) ∈ Type_Num 
+      ∀ Γ Σ z, 
+      has_type Σ Γ  (E_Num z)  Type_Num  
 
   | T_Minus : 
-      ∀ Γ e1 e2, 
-      Γ ⊢ e1 ∈ Type_Num ->
-      Γ ⊢ e2 ∈ Type_Num ->
-      Γ ⊢ (E_Minus e1 e2) ∈ Type_Num 
+      ∀ Γ Σ e1 e2, 
+      has_type Σ Γ  e1  Type_Num -> 
+      has_type Σ Γ  e2  Type_Num -> 
+      has_type Σ Γ  (E_Minus e1 e2)  Type_Num  
     
   | T_Eq :
-      ∀ Γ e1 e2, 
-      Γ ⊢ e1 ∈ Type_Num ->
-      Γ ⊢ e2 ∈ Type_Num ->
-      Γ ⊢ (E_Eq e1 e2) ∈ Type_Bool 
+      ∀ Γ Σ e1 e2, 
+      has_type Σ Γ  e1  Type_Num -> 
+      has_type Σ Γ  e2  Type_Num -> 
+      has_type Σ Γ  (E_Eq e1 e2)  Type_Bool  
 
   (* Pairs *)
   | T_Pair :
-      ∀ Γ e₁ e₂ t₁ t₂, 
-      Γ ⊢ e₁ ∈ t₁ ->
-      Γ ⊢ e₂ ∈ t₂ ->
-      Γ ⊢ (E_Pair e₁ e₂) ∈ (Type_Prod t₁ t₂) 
+      ∀ Γ Σ e₁ e₂ t₁ t₂, 
+      has_type Σ Γ  e₁  t₁ -> 
+      has_type Σ Γ  e₂  t₂ -> 
+      has_type Σ Γ  (E_Pair e₁ e₂)  (Type_Prod t₁ t₂)  
   | T_First :
-      ∀ Γ e t₁ t₂,
-      Γ ⊢ e ∈ (Type_Prod t₁ t₂) ->
-      Γ ⊢ (E_First e) ∈ t₁
+      ∀ Γ Σ e t₁ t₂,
+      has_type Σ Γ  e  (Type_Prod t₁ t₂) -> 
+      has_type Σ Γ  (E_First e)  t₁ 
   | T_Second :
-      ∀ Γ e t₁ t₂,
-      Γ ⊢ e ∈ (Type_Prod t₁ t₂) ->
-      Γ ⊢ (E_Second e) ∈ t₂
+      ∀ Γ Σ e t₁ t₂,
+      has_type Σ Γ  e  (Type_Prod t₁ t₂) -> 
+      has_type Σ Γ  (E_Second e)  t₂ 
 
   (* Records *)
   | T_Record_Nil :
-      ∀ Γ, 
-      Γ ⊢ E_Record_Nil ∈ Type_Record_Nil
+      ∀ Γ Σ, 
+      has_type Σ Γ  (E_Record_Nil)  (Type_Record_Nil) 
   | T_Record_Cons :
-      ∀ Γ x e tail t_e t_tail, 
-      Γ ⊢ e ∈ t_e -> 
-      Γ ⊢ tail ∈ t_tail -> 
-      record_type t_tail -> 
-      Γ ⊢ (E_Record_Cons x e tail) ∈ (Type_Record_Cons x t_e t_tail) 
+      ∀ Γ Σ x e t_e e_tail t_tail, 
+      has_type Σ Γ  e  t_e ->  
+
+      has_type Σ Γ  e_tail  t_tail ->  
+      record_type t_tail ->
+      has_type Σ Γ  (E_Record_Cons x e e_tail)  (Type_Record_Cons x t_e t_tail)  
   | T_Record_Access :
-      ∀ Γ x e t_e t_acc, 
-      Γ ⊢ e ∈ t_e -> 
+      ∀ Γ Σ x e t_e t_acc, 
+      has_type Σ Γ  e  t_e ->  
       lookup_type_record x t_e = Some t_acc ->
-      Γ ⊢ (E_Record_Access e x) ∈ t_acc
+      has_type Σ Γ  (E_Record_Access e x)  t_acc 
   
   | T_Fix :
-      ∀ Γ e t, 
-      Γ ⊢ e ∈ (Type_Fun t t) -> 
-      Γ ⊢ (E_Fix e) ∈ t
-  where
-    "Γ '⊢' e '∈' τ" := (has_type Γ e τ)
+      ∀ Γ Σ e t, 
+      has_type Σ Γ  e (Type_Fun t t) ->  
+      has_type Σ Γ  (E_Fix e)  t 
+
+  (* Sum types *)
+  | T_Unit : ∀ Γ Σ, has_type Σ Γ E_Unit (Type_Unit)  
+  | T_In_Left :
+      ∀ Γ Σ t₁ t₂ e, 
+      has_type Σ Γ  e  t₁ ->  
+      has_type Σ Γ  (E_In_Left t₁ t₂ e)  (Type_Disjoint_Union t₁ t₂) 
+  | T_In_Right :
+      ∀ Γ Σ t₁ t₂ e, 
+      has_type Σ Γ  e  t₂ ->  
+      has_type Σ Γ  (E_In_Right t₁ t₂ e)  (Type_Disjoint_Union t₁ t₂) 
+  | T_Match :
+      ∀ Γ Σ t₁ t₂ tf e e_left e_right, 
+      has_type Σ Γ e (Type_Disjoint_Union t₁ t₂) ->  
+      has_type Σ Γ e_left  (Type_Fun t₁ tf) -> 
+      has_type Σ Γ e_right  (Type_Fun t₂ tf) -> 
+      has_type Σ Γ (E_Match e e_left e_right) tf 
+
+  | T_Sum_Constr: 
+      ∀ Γ Σ e constr name t,
+      lookup_type_sum constr Σ = Some (name, t) -> 
+      has_type Σ Γ e t ->
+      has_type Σ Γ (E_Sum_Constr constr e) (Type_Sum name)
+
+  (* | T_Sum_Match :
+      ∀ Σ Γ e name branches,
+      has_type Σ Γ e (Type_Sum name) ->
+      ( 
+        ∀ e, 
+        In e branches ->
+        ∀ name e_branch exp_t,
+        expected_parameter (name, e_branch, exp_t)
+      
+      ) *)
+
+
+
+  | T_Exception :
+      ∀ Σ Γ e t,
+      has_type Σ Γ (E_Exception e) t
 .
 
 Hint Constructors has_type : local_hints.
 
-  
-  
-Local Lemma weakening : ∀ Γ Γ' e t, 
+
+
+Local Lemma weakening : ∀ Γ Γ' Σ e t, 
   Maps.includedin Γ Γ' ->
-  Γ ⊢ e ∈ t ->
-  Γ' ⊢ e ∈ t.
+  has_type Σ Γ e t -> 
+  has_type Σ Γ' e t. 
 Proof.
   intros * H_included H_type.
   generalize dependent Γ'.
@@ -131,9 +205,9 @@ Qed.
 Hint Resolve weakening : local_hints.
 
 
-Local Lemma weakening_empty : ∀ Γ e t, 
-  empty ⊢ e ∈ t ->
-  Γ ⊢ e ∈ t.
+Local Lemma weakening_empty : ∀ Γ Σ e t, 
+  has_type Σ empty  e  t -> 
+  has_type Σ Γ e t. 
 Proof.
   intros. apply (weakening empty); auto.
   intros x v contra. discriminate contra.
