src/Canonical_form.v
@@ -2,13 +2,16 @@ From Coq Require Import Unicode.Utf8.
 Require Import Hints.
 Require Import Syntax.
 Require Import Types.
+Local Open Scope Z_scope.
+Require Import ZArith.
 Require Maps.
+Import Maps.Notations.
 
 Local Lemma t_num : 
-    ∀ Γ e,
-    Γ ⊢ e ∈ Type_Num -> 
+    ∀ Γ Σ e,
+    has_type Σ Γ  e  Type_Num ->  
     value e ->
-    ∃ z, e = E_Num z.
+    ∃ (z : Z), e = <{z}>.
 Proof.
     intros * H_type H_val.
     inversion H_val; eauto; 
@@ -18,10 +21,10 @@ Qed.
 Hint Resolve t_num : local_hints.
 
 Local Lemma t_bool : 
-    ∀ Γ e,
-    Γ ⊢ e ∈ Type_Bool -> 
+    ∀ Γ Σ e,
+    has_type Σ Γ  e  Type_Bool ->  
     value e ->
-    e = E_True \/ e = E_False.
+    e = <{true}> \/ e = <{false}>.
 Proof.
     intros * H_type H_val.
     inversion H_val; subst; auto;
@@ -31,10 +34,10 @@ Qed.
 Hint Resolve t_bool : local_hints.
 
 Local Lemma t_fun : 
-    ∀ Γ e t1 t2,
-    Γ ⊢ e ∈ (Type_Fun t1 t2) -> 
+    ∀ Γ Σ e t1 t2,
+    has_type Σ Γ  e  (Type_Fun t1 t2) ->  
     value e ->
-    ∃ x e', e = E_Fun x t1 e'. 
+    ∃ x e', e = <{fun x : t1 => e'}>. 
 Proof.
     intros * H_type H_val.
     inversion H_val; subst; try (inversion H_type; fail).
@@ -45,10 +48,10 @@ Hint Resolve t_fun : local_hints.
 
 
 Local Lemma t_pair :
-    ∀ Γ e t₁ t₂,
-    Γ ⊢ e ∈ (Type_Prod t₁ t₂) -> 
+    ∀ Γ Σ e t₁ t₂,
+    has_type Σ Γ  e  (Type_Prod t₁ t₂) ->  
     value e ->
-    ∃ e₁ e₂, e = E_Pair e₁ e₂.
+    ∃ e₁ e₂, e = <{(e₁, e₂)}>.
 Proof.
     intros * H_type H_val.
     inversion H_val; subst; try (inversion H_type; fail).
@@ -58,10 +61,10 @@ Hint Resolve t_pair : local_hints.
 
 
 Local Lemma t_record_nil :
-    ∀ Γ e,
-    Γ ⊢ e ∈ Type_Record_Nil -> 
+    ∀ Γ Σ e,
+    has_type Σ Γ  e  (Type_Record_Nil) ->  
     value e ->
-    e = E_Record_Nil.
+    e = <{nil}>.
 Proof.
     intros * H_type H_val.
     inversion H_val; subst; try (inversion H_type; fail).
@@ -72,8 +75,8 @@ Hint Resolve t_record_nil : local_hints.
 
 
 Local Lemma t_record_cons :
-    ∀ Γ e x t_x t_tail,
-    Γ ⊢ e ∈ (Type_Record_Cons x t_x t_tail) -> 
+    ∀ Γ Σ e x t_x t_tail,
+    has_type Σ Γ  e  (Type_Record_Cons x t_x t_tail) ->  
     value e ->
     ∃ e' e_tail, e = E_Record_Cons x e' e_tail.
 Proof.
@@ -86,25 +89,25 @@ Hint Resolve t_record_cons : local_hints.
 
 
 Local Lemma record_type_exists :
-  ∀ Γ e t_rec t x, 
+  ∀ Γ Σ e t_rec t x, 
   value e ->
-  Γ ⊢ e ∈ t_rec ->
+  has_type Σ Γ  e  t_rec -> 
   lookup_type_record x t_rec = Some t -> 
   ∃ e', lookup_val_record x e = Some e'.
 Proof.
-  intros Γ e t_rec.
+  intros Γ Σ e t_rec.
   generalize dependent Γ.
   generalize dependent e.
   induction t_rec; intros;
   try (inversion H1; fail).
-  simpl in H1.
+  simpl in H1. 
   assert (H2 := H0). 
-  apply t_record_cons in H0 as [e' [e_tail H_eq]]; 
+  apply t_record_cons in H0 as [e' [e_tail H_eq]];
   subst; eauto. 
   simpl.
-  destruct (String.eqb_spec x0 x); eauto.
+  destruct (String.eqb_spec x0 x); subst; eauto.
   inversion H; subst.
-  inversion H2.
+  inversion H2; subst.
   eapply IHt_rec2; eauto.
 Qed.
 
@@ -112,14 +115,14 @@ Hint Resolve record_type_exists : local_hints.
 
 
 Lemma lookup_type_val :
-  ∀ Γ x e e' t_e t_e',
-  Γ ⊢ e ∈ t_e ->
+  ∀ Γ Σ x e e' t_e t_e',
+  has_type Σ Γ  e  t_e -> 
   value e ->
   lookup_type_record x t_e = Some t_e' ->
   lookup_val_record x e = Some e' -> 
-  Γ ⊢ e' ∈ t_e'.
+  has_type Σ Γ  e'  t_e'. 
 Proof.
-  intros Γ x e e' t_e.
+  intros Γ Σ x e e' t_e.
   generalize dependent Γ. 
   generalize dependent x. 
   generalize dependent e. 
@@ -140,7 +143,7 @@ Proof.
     subst.
     inversion H_val; subst.
     inversion H; subst.
-    eapply IHt_e2; 
+    eapply IHt_e2;
     eauto;
     simpl in *;
     rewrite <- String.eqb_neq in n;
@@ -150,3 +153,35 @@ Proof.
 Qed.
 
 Hint Resolve lookup_type_val : local_hints.
+
+
+Local Lemma t_in: 
+    ∀ Γ Σ e t₁ t₂,
+    has_type Σ Γ  e  (Type_Disjoint_Union t₁ t₂) ->  
+    value e ->
+    ∃ e', e = E_In_Left t₁ t₂ e' \/ e = E_In_Right t₁ t₂ e'.
+Proof.
+    intros * H_type H_val.
+    inversion H_val; subst; inversion H_type; subst;
+    eauto.
+Qed.
+Hint Resolve t_in : local_hints.
+
+
+Local Lemma t_enum :
+    ∀ Γ Σ e name,
+    has_type Σ Γ e (Type_Sum name) ->  
+    value e ->
+    ∃ constr e' t, 
+       lookup_type_sum constr Σ = Some (name, t)
+    /\ has_type Σ Γ e' t
+    /\ e = E_Sum_Constr constr e'.
+Proof.
+  intros * H_type H_val.
+  inversion H_val; subst; inversion H_type; subst. 
+  eauto 6.
+Qed.
+  
+
+Hint Resolve t_enum : local_hints.
+
