src/Eval.v
@@ -1,0 +1,407 @@
+From Coq Require Import Unicode.Utf8.
+Require Import Types.
+Require Import Syntax.
+Require Import Step.
+Require Import Subst.
+Require Import Hints.
+Require Import Closed.
+Local Open Scope Z_scope.
+Require Import ZArith.
+Require Import Lia.
+Require Import String.
+Require Import Multi.
+(* TODO éventuellement: lien avec multistep *)
+
+Fixpoint sub (s : expr) (x : string) (e: expr) := 
+  match e with 
+  | E_Var v => if (x =? v)%string then s else E_Var v
+
+  | <{ e₁ e₂}> => 
+      let e₁ := sub s x e₁ in
+      let e₂ := sub s x e₂ in
+      <{e₁ e₂}>
+
+  | <{fun v : t => e}> => 
+      let e :=
+        if (x =? v)%string 
+        then e
+        else sub s x e 
+      in
+      <{fun v : t => e}>
+
+  | <{true}> => <{true}>
+
+  | <{false}> => <{false}>
+
+  | <{if e₁ then e₂ else e₃}> => 
+      let e₁ := sub s x e₁ in
+      let e₂ := sub s x e₂ in
+      let e₃ := sub s x e₃ in
+      <{if e₁ then e₂ else e₃}>
+
+  | <{let v = e₁ in e₂}> =>
+      let e₁ := sub s x e₁ in
+      let e₂ :=
+        if (x =? v)%string 
+        then e₂
+        else sub s x e₂  in
+      <{let v = e₁ in e₂}>
+
+  | E_Num z => E_Num z
+
+  | <{ e₁ - e₂}> => 
+      let e₁ := sub s x e₁ in
+      let e₂ := sub s x e₂ in
+      <{e₁ - e₂}>
+
+  | <{ e₁ == e₂}> => 
+      let e₁ := sub s x e₁ in
+      let e₂ := sub s x e₂ in
+      <{e₁ == e₂}>
+
+  | <{(e₁, e₂)}> =>
+      let e₁ := sub s x e₁ in
+      let e₂ := sub s x e₂ in
+      <{(e₁, e₂)}>
+
+  | <{first e}> => 
+      let e := sub s x e in
+      <{first e}>
+
+  | <{second e}> => 
+      let e := sub s x e in
+      <{second e}>
+
+  | <{nil}> => <{nil}>
+
+  | <{ v := e; etail}> => 
+      let e := sub s x e in
+      let etail := sub s x etail in
+      <{ v := e; etail}>
+  | <{e::v}> =>
+      let e := sub s x e in
+      <{e :: v}>
+  | <{fix e}> =>
+      let e := sub s x e in
+      <{fix e}>
+
+  | E_In_Left t₁ t₂ e => E_In_Left t₁ t₂ (sub s x e)
+  | E_In_Right t₁ t₂ e => E_In_Right t₁ t₂ (sub s x e)
+  | E_Match e e_left e_right => E_Match (sub s x e) (sub s x e_left) (sub s x e_right)
+  | E_Unit => E_Unit
+  | E_Sum_Constr constr e => E_Sum_Constr constr (sub s x e)
+  end.
+
+Inductive result {A B} := 
+  | Ok : A -> result 
+  | Err : B ->  result
+. 
+Fixpoint eval_aux (n : nat) (e : expr) : @result expr string   := 
+  match n with 
+  | O => Err "Maximum recursion depth reached"%string
+  | S n => 
+    match e with 
+    | E_Var x => Err ("Unbound variable" ++ x)%string 
+    | <{ e₁ e₂}> => 
+      match eval_aux n e₁ with 
+      | Ok <{fun x : t => e}> => eval_aux n (sub e₂ x e)
+      | Ok _ => Err "Non-functional appplication"%string
+      | e => e
+      end
+    | <{fun x : t => e}> => Ok <{fun x : t => e}>
+    | <{true}> => Ok <{true}>
+    | <{false}> => Ok <{false}>
+    | <{if e₁ then e₂ else e₃}> => 
+      match eval_aux n e₁ with 
+      | Ok <{true}> => eval_aux n e₂
+      | Ok <{false}> => eval_aux n e₃
+      | Ok _ => Err "Non-boolean If condition"%string
+      | err => err
+      end
+    | <{let x = e₁ in e₂}> => eval_aux n (sub e₁ x e₂)
+    | E_Num z => Ok (E_Num z)
+    | <{ e₁ - e₂}> => 
+      match eval_aux n e₁, eval_aux n e₂ with 
+      | Ok (E_Num z₁), Ok (E_Num z₂) => Ok (E_Num (z₁ - z₂))
+      | Ok _, Ok _ => Err "Non Numeric substraction"%string
+      | Err e, _ | _, Err e => Err e
+      end
+    | <{ e₁ == e₂}> => 
+      match eval_aux n e₁, eval_aux n e₂ with 
+      | Ok (E_Num z₁), Ok (E_Num z₂) => Ok (
+        if z₁ =? z₂ then <{true}> else <{false}>
+      )
+      | Ok _, Ok _ => Err "Non Numeric comparison"%string
+      | Err e, _ | _, Err e => Err e
+      end
+
+    | <{(e₁, e₂)}> =>
+      match eval_aux n e₁, eval_aux n e₂ with 
+      | Ok e₁, Ok e₂ => Ok <{e₁, e₂}>
+      | Err e, _  | _, Err e => Err e
+      end
+
+  | <{first e}> => 
+      match eval_aux n e with 
+      | Ok <{ e₁, _ }> => Ok e₁
+      | Ok _ => Err "Non pair projection first"%string
+      | e => e
+      end
+
+  | <{second e}> => 
+      match eval_aux n e with 
+      | Ok <{ _, e₂ }> => Ok e₂
+      | Ok _ => Err "Non pair projection second"%string
+      | e => e
+      end
+
+  | <{nil}> => Ok <{nil}>
+
+  | <{ x := e; etail}> => 
+      match eval_aux n e, eval_aux n etail with 
+      | Ok e, Ok etail => Ok <{ x := e; etail}>
+      | Err e, _ | _, Err e => Err e
+      end 
+  | <{e::x}> =>
+      match eval_aux n e with 
+      | Ok e => 
+        match lookup_val_record x e with 
+        | Some e => Ok e 
+        | None =>  Err ("Access to unbound field " ++ x ++ " or to a non-record value")%string
+        end
+      | err => err
+      end
+  | <{fix e}> =>
+      match eval_aux n e with 
+      | Ok <{fun x : t => e}> => 
+        let e := sub <{fix <{fun x : t => e}>}> x e in 
+        Ok e
+      | err => err 
+      end
+  | E_In_Left t₁ t₂ e =>
+      match eval_aux n e with 
+      | Ok e => Ok (E_In_Left t₁ t₂ e)
+      | err => err
+      end
+  | E_In_Right t₁ t₂ e =>
+      match eval_aux n e with 
+      | Ok e => Ok (E_In_Right t₁ t₂ e)
+      | err => err
+      end
+  | E_Match e e_left e_right =>
+      match eval_aux n e with 
+      | Ok (E_In_Left _ _ e) => eval_aux n (E_App e_left e)
+      | Ok (E_In_Right _ _ e) => eval_aux n (E_App e_right e)
+      | err => err
+      end
+  | E_Unit => Ok E_Unit
+  | E_Sum_Constr constr e =>
+    match eval_aux n e with 
+    | Ok e' => Ok (E_Sum_Constr constr e')
+    | err => err
+    end
+  end
+end.
+
+Definition eval := eval_aux (5001)%nat. 
+
+
+Definition eq := "eq"%string.
+Definition m := "m"%string.
+Definition n := "n"%string.
+
+Compute eval <{
+  let eq = fix
+    fun eq : (Type_Num -> Type_Num -> Type_Bool) =>
+      fun m : Type_Num => 
+        fun n : Type_Num => 
+          if m == 0
+          then n == 0 
+          else 
+            if n == 0 
+            then false 
+            else  
+              eq (n-1) (m-1)
+  in 
+  let n = 10 in 
+  let m = 10 in 
+  eq n m
+}>.
+
+
+
+Definition add := 
+  let n := "n"%string in 
+  let m := "m"%string in 
+  <{fun n : Type_Num => fun m : Type_Num => n - (0 - m)}>.
+
+
+Definition mul := 
+  let n := "n"%string in 
+  let m := "m"%string in 
+  let mul := "mul"%string in 
+  <{
+    fix 
+      fun mul : Type_Num -> Type_Num -> Type_Num => 
+      fun n : Type_Num =>
+      fun m : Type_Num =>
+        if n == 0 
+        then 0 
+        else add m (mul m (n - 1))
+  }>.
+
+Definition fact := 
+  let fact := "fact"%string in 
+  <{
+    fix 
+      fun fact : Type_Num -> Type_Num =>
+      fun n : Type_Num => 
+      if n == 0 then 1 
+      else mul n (fact (n-1))
+  }>
+
+.
+
+
+Compute eval <{fact 5}>.
+
+Definition div2 :=
+  let div2 := "div2"%string in 
+ <{
+  fix 
+    fun div2 : Type_Num -> Type_Num -> Type_Num =>
+    fun n : Type_Num => 
+    if n == 0 then 0 
+    else 
+      if n == 1
+      then 0 
+      else add 1 (div2 (n - 2))
+ }>.
+
+
+Definition sumrec := 
+  let sumrec := "sumrec"%string in 
+  <{
+    fix 
+      fun sumrec : Type_Num -> Type_Num =>
+      fun n : Type_Num =>
+      if n == 0 then 0 
+      else add n (sumrec (n - 1)) 
+  }>
+  .
+
+Definition sumcalc := 
+  let sumcalc := "sumcalc"%string in 
+  <{
+    fun n : Type_Num => div2 (mul n (add n 1)) 
+  }>.
+Compute eval <{
+  sumcalc 18 == sumrec 18
+}>.
+
+
+Theorem substitution_sub :
+  ∀ s x e e',
+  closed s ->
+  substitution s x e e' <->
+  sub s x e = e'.
+Proof with eauto with local_hints.
+  split.
+  {
+  generalize dependent s; 
+  generalize dependent x; 
+  generalize dependent e'.
+  induction e; intros * H_closed H_subst; 
+  try 
+  (
+    simpl;
+    inversion H_subst; subst;
+    try apply IHe in H0;
+    try apply IHe in H2;
+    try apply IHe1 in H1;
+    try apply IHe2 in H3;
+    try apply IHe1 in H4;
+    try apply IHe2 in H3;
+    subst;
+    eauto with local_hints;
+    fail
+  ).
+  - simpl. destruct (String.eqb_spec x0 x); 
+    inversion H_subst; subst;
+    eauto; exfalso...
+  - simpl. destruct (String.eqb_spec x0 x); 
+    inversion H_subst; subst; 
+    try (exfalso; eauto with local_hints; fail)...
+    apply IHe in H5; subst...
+  - simpl.
+    inversion H_subst; subst.
+    apply IHe1 in H2;
+    apply IHe2 in H4;
+    apply IHe3 in H5;
+    subst;
+    eauto with local_hints.
+  - simpl. 
+    simpl. destruct (String.eqb_spec x0 x); 
+    inversion H_subst; subst;
+    try (exfalso; eauto with local_hints; fail)...
+    apply IHe1 in H3; subst...
+    apply IHe1 in H5; apply IHe2 in H6; subst...
+  - simpl. inversion H_subst; subst. erewrite IHe.
+    + reflexivity.
+    + assumption.
+    + assumption.  
+  - simpl. inversion H_subst; subst. erewrite IHe.
+    + reflexivity.
+    + assumption.
+    + assumption. 
+  - simpl. inversion H_subst; subst. 
+    erewrite IHe1; try erewrite IHe2; try erewrite IHe3; auto.
+  }
+  {
+  generalize dependent s; 
+  generalize dependent x; 
+  generalize dependent e'.
+  induction e; intros * H_closed H_subst;
+  simpl in H_subst;
+  try (
+      try destruct (String.eqb_spec x0 x); 
+      inversion H_subst; subst; 
+      eauto with local_hints; fail
+  ).
+  }
+Qed.
+
+Theorem eval_value :
+  ∀ e e' n,
+  eval_aux n e = Ok e' ->
+  value e'.
+Proof.
+  intros e.
+  induction e; intros e' n H_eval; destruct n;
+  try (inversion H_eval; fail); simpl in H_eval.
+  - destruct (eval_aux n0 e1);
+    try destruct e; try (inversion H_eval; fail).
+  (* Faux, il faut bien typer *)
+    
+
+Admitted.
+
+Theorem eval_multistep :
+  ∀ Σ e t e' n, 
+  has_type Σ empty e t ->
+  eval_aux n e = Ok e' ->
+  e -->* e'.
+Proof with eauto with local_hints.
+  induction e; intros.
+  - destruct n0;
+    inversion H0.
+  - destruct n0. inversion H0.
+    simpl in H0.
+    destruct (eval_aux n0 e1).
+    + destruct e; try (inversion H0; fail).
+      inversion H; subst.
+    
+      
+
+Admitted.
+
