src/Preservation.v
@@ -15,20 +15,28 @@ Import Maps.Notations.
 
 
 
-Theorem preservation : ∀ e e' t,
-  empty ⊢ e ∈ t  ->
-  e ->> e'  ->
-  empty ⊢ e' ∈ t.
+Theorem preservation : ∀ Σ e e' t,
+  has_type Σ empty e t  ->
+  e --> e'  ->
+  has_type Σ empty e' t.
 Proof.
   intros * H_type_e. 
   generalize dependent e'.
   remember empty as Γ.
-  induction H_type_e;   
-  intros e' H_step;  
+  induction H_type_e;
+  intros e' H_step.
+  21: {
+    (* e = E_Match e' e_left e_right *)
+    inversion H_step; subst; 
+    inversion H_type_e1; subst;
+      eauto with local_hints.
+  }
+  all :
   try (
     inversion H_step; 
     subst; 
     try inversion H_type_e; subst;
+    (* try inversion H_type_e1; subst; *)
     try inversion H_type_e2; subst;
     eauto with local_hints; fail
   ).
