test.v
@@ -1,0 +1,121 @@
+(*
+  Tight Typings and Split Bounds,
+    BENIAMINO ACCATTOLI
+    STÉPHANE GRAHAM-LENGRAND
+    DELIA KESNER
+  https://arxiv.org/pdf/1807.02358.pdf
+*)
+From Coq Require Import Unicode.Utf8.
+
+
+Require Import String.
+Require Import Arith.
+From Coq Require Import Unicode.Utf8.
+
+
+Inductive term : Set :=
+  | T_Var (n : nat)
+  | T_App (t₁ t₂ : term)
+  | T_Abs (t : term)
+.
+
+Declare Custom Entry term.
+Notation "<{ e }>" := e (e custom term at level 99).
+ Notation "( x )" := x (in custom term, x at level 99).
+Notation "'`' e '`'" := e (in custom term at level 0, e constr).
+Notation "x" := x (in custom term at level 0, x constr at level 0).
+Notation "'#' n" := (T_Var n) (in custom term at level 0).
+ Notation "x y" := (T_App x y) (in custom term at level 1, left associativity).
+Notation "'λ' t" := (T_Abs t) (
+  in custom term at level 90, 
+  t custom term at level 99,
+  left associativity
+).
+
+Check <{ (λ #0 #0)(λ #0 #0) }>.
+
+Fixpoint incr_indices (n : nat) (t : term) : term :=
+  match t with
+  | <{#v}> => if v <? n then <{#v}> else <{#`v+n`}>
+  | <{λ t}> => <{λ `incr_indices n t`}>
+  | <{t1 t2}> => <{`incr_indices n t1` `incr_indices n t2`}>
+  end.
+
+Search (nat -> nat -> bool).
+
+Reserved Notation "t '[' n ':=' s ']'" (in custom term at level 99, s at level 99).
+
+Fixpoint subst (n : nat) (s : term) (t : term) : term :=
+  match t with 
+  | <{#v}> => 
+      if (n =? v)%nat 
+      then s
+      else if (v <? n) 
+            then <{#v}>
+            else <{#`v - 1`}>
+  | <{λ t}> => <{λ `subst (n+1) (incr_indices 1 s) t`}>
+  | <{t1 t2}> => <{t1[n := s] t2[n:=s]}>
+  end
+  where "t '[' n ':=' s ']'" := (subst n s t) (in custom term at level 99, s at level 99).
+
+
+
+Check <{ λ λ ((λ #2 #1 #0) (λ #0))  }>.
+
+Eval simpl in <{(λ λ (#2 #1 #0 [0 := λ #0]))}>.
+
+
+
+Definition deterministic {A} (relation : A -> A -> Prop) : Prop :=
+  ∀ a a₁ a₂, relation a a₁ -> relation a a₂ -> a = a₂. 
+
+Definition rel_normal {A} (relation : A -> A -> Prop) (a : A) : Prop := 
+  ¬ ∃ b, relation a b.
+
+(* 
+  Definition 2.1 (Evaluation system)
+ *)
+
+Section EvalSystem.
+Variable T : Set.
+Variable relation : T -> T -> Prop.
+Variable (normal neutral abs : T -> Prop).
+
+Definition evaluation_system : Prop :=
+        deterministic relation
+    /\  (∀ t, rel_normal relation t <-> normal t) 
+    /\  (∀ t, neutral t <-> (normal t /\ ¬ abs t))
+.
+
+End EvalSystem.
+
+Check evaluation_system.
+
+
+Inductive reflexive_closure {A} (rel : A -> A -> Prop) : A -> A -> Prop :=
+  | RC_refl : ∀ t, reflexive_closure rel t t 
+  | RC_self : ∀ t₁ t₂,
+    rel t₁ t₂ -> 
+    reflexive_closure rel t₁ t₂
+.
+
+Inductive transitive_closure {A} (rel : A -> A -> Prop) : A -> A -> Prop := 
+  | TC_self :  
+      ∀ t₁ t₂,
+      rel t₁ t₂ -> 
+      transitive_closure rel t₁ t₂
+  | TC_trans :
+      ∀ t₁ t₂ t₃, 
+      transitive_closure rel t₁ t₂ ->
+      transitive_closure rel t₂ t₃ ->
+      transitive_closure rel t₁ t₃
+.
+
+Inductive n_iteration {A} (rel : A -> A -> Prop) : nat -> A -> A -> Prop := 
+  | NI_O : ∀ t, n_iteration rel O t t 
+  | NI_Sn : 
+      ∀ n t₁ t₂ t₃, 
+      rel t₁ t₂ -> 
+      n_iteration rel n t₂ t₃ ->
+      n_iteration rel (S n) t₁ t₃
+.
